set.v
@@ -1,29 +1,32 @@
-Module TAPL_Set.
-
-From Ssreflect Require Import ssreflect.
+From mathcomp Require Import ssreflect.
 Require Import MSets Equalities.
+
+Module TAPL_Set.
 
 Module SetNotation (E:DecidableType) (Import S:WSetsOn E).
 
-  Notation " { } " := empty (format "{ }", at level 0).
-  Notation " { x } " := (add x empty).
-  Notation " { x ; .. ; y } " := (add x .. (add y empty) ..).
+  Notation " {{ }} " := empty (at level 100) : set_scope.
+  Notation " {{ x }} " := (add x empty) (at level 100) : set_scope.
+  Notation " {{ x ; .. ; y }} " := (add x .. (add y empty) ..) (at level 100) : set_scope.
 
-  Notation " x @ s " := ((mem x s) = true) (at level 90, no associativity).
-  Notation " x @? s " := (mem x s) (at level 90, no associativity).
+  Notation " x @ s " := ((mem x s) = true) (at level 90, no associativity) : set_scope.
+  Notation " x @? s " := (mem x s) (at level 90, no associativity) : set_scope.
+ 
+  Notation " x :: s " := (add x s) (at level 60, right associativity) : set_scope.
+  Notation " x \/ y " := (union x y) (at level 85, right associativity) : set_scope.
+  Notation " x /\ y " := (inter x y) (at level 80, right associativity) : set_scope.
+  Notation " x \ y " := (diff x y) (at level 60, no associativity) : set_scope.
 
-  Notation " x :: s " := (add x s) (at level 60, right associativity).
-  Notation " x \/ y " := (union x y) (at level 85, right associativity).
-  Notation " x /\ y " := (inter x y) (at level 80, right associativity).
-  Notation " x \ y " := (diff x y) (at level 60, no associativity).
+  Notation " # x " := (cardinal x) (at level 35, x at next level) : set_scope.
 
-  Notation " # x " := (cardinal x) (at level 35, x at next level).
+  Delimit Scope set_scope with set.
 
 End SetNotation.
 
 Module SetExt (E:DecidableType) (Import S:WSetsOn E).
   Module Notations := SetNotation E S.
   Import Notations.
+  Local Open Scope set_scope.
 
   Lemma cardinal_union : forall (s1 s2 : t), #(s1 \/ s2) <= #s1 + #s2.
   Admitted.
@@ -52,22 +55,27 @@ Module Ex_Inductive.
   Notation bool_set := BoolSet.t.
   Import BoolSetNotation.
 
-  Check {}.
-  Check {t; f}.
-  Eval compute in #{t; t; f}.
-  Eval compute in #({t; t; f} \ {t}).
+  Section NotationCheck.
+    Local Open Scope set_scope.
+
+    Check {{}}.
+    Check {{t; f}}.
+    Eval compute in #{{t; t; f}}.
+    Eval compute in #({{t; t; f}} \ {{t}}).
+
+  End NotationCheck.
 
 End Ex_Inductive.  
 
 Module NatSetNotation (E:OrderedType) (Import S:WSetsOn E).
 
-  Notation " { } " := empty (format "{ }", at level 0) : nat_nat_set_scope.
-  Notation " { x } " := (add x empty) : nat_set_scope.
-  Notation " { x ; .. ; y } " := (add x .. (add y empty) ..) : nat_set_scope.
+  Notation " {{ }} " := empty (at level 100) : nat_set_scope.
+  Notation " {{ x }} " := (add x empty) (at level 100) : nat_set_scope.
+  Notation " {{ x ; .. ; y }} " := (add x .. (add y empty) ..) (at level 100) : nat_set_scope.
 
   Notation " x @ s " := ((mem x s) = true) (at level 90, no associativity) : nat_set_scope.
   Notation " x @? s " := (mem x s) (at level 90, no associativity) : nat_set_scope.
-
+ 
   Notation " x :: s " := (add x s) (at level 60, right associativity) : nat_set_scope.
   Notation " x \/ y " := (union x y) (at level 85, right associativity) : nat_set_scope.
   Notation " x /\ y " := (inter x y) (at level 80, right associativity) : nat_set_scope.
@@ -75,13 +83,14 @@ Module NatSetNotation (E:OrderedType) (Import S:WSetsOn E).
 
   Notation " # x " := (cardinal x) (at level 35, x at next level) : nat_set_scope.
 
+  Delimit Scope nat_set_scope with nat_set.
+
 End NatSetNotation.
 
 Module NatSet := MSetList.Make PeanoNat.Nat.
 Module NatSetNotationM := NatSetNotation PeanoNat.Nat NatSet.
 
 Notation nat_set := NatSet.t.
-Delimit Scope nat_set_scope with nat_set.
 
 Export MSets Equalities NatSetNotationM.
 
